

Nuclear matter EoS with minimal length  
( $\sigma(\omega)$ -model)

Minimal length  $\Rightarrow$  Komutasi field operator harus bersikap non-lokal

$$\delta(\vec{x}-\vec{y}) \longrightarrow \tilde{\delta}(\vec{x}-\vec{y}) = \frac{1}{\pi(\vec{x}-\vec{y})} \sin \left[ \frac{\pi(\vec{x}-\vec{y})}{2\ell_b \sqrt{\beta}} \right]$$

Referensi Utama:

- 1) Kh. Nouvier, J. Phys. A: Math. Gen 38 (2005)
- 2) Frassino-Panella, PRD 85 (2012), 045030
- 3) Panella, PRD 76, 045012 (2007)

(1) Momentum modified to (to all orders in  $\beta$ ):

$$p_i \longrightarrow \bar{p}_i(p) = \frac{1}{\sqrt{\beta} p} \left[ \tan^{-1}(\sqrt{\beta} p) \right] p_i \quad \dots (1)$$

(2) GUP  $\oplus$  Dirac equation (in momentum rep):

$$(\gamma^\mu \bar{p}_\mu - m^*) \psi(p) = 0 \quad \dots (2)$$

(3) State "plane-wave" = Maximized localized state:

$$\psi(\vec{x}, t) = A e^{-i(\omega_p t - \vec{p} \cdot \vec{x})} \quad \dots (3)$$

(4) Dispersion relation

from (2) one will get:

$$(p_0)^2 - \bar{p}^2 - m^{*2} = 0$$

$$\omega_p^2 = \bar{p}^2 + m^{*2}$$

$$\omega_p^2 = \frac{1}{\beta} \left[ \tan^{-1} \sqrt{\beta} p \right]^2 + m^{*2} \quad \dots (4)$$

①

(5) Normalisation Condition Yang disubstitusikan

$$\sum_{\alpha=1}^2 U^\dagger(\vec{p}, \alpha) U(\vec{p}, \alpha) = 2$$

$$\sum_{\alpha=1}^2 \bar{U}(\vec{p}, \alpha) U(\vec{p}, \alpha) = \frac{2m^*}{\omega_p} \quad \dots (5)$$

(6) Field operator (2nd Quantization with GUE)

expand in maximally localized state

$$\psi(\vec{x}, t) = \sum_{\alpha} \int \frac{d^3 p}{(1+p^2)(2\pi)^3} N_p \left[ b(\vec{p}, \alpha) e^{i(-\vec{p} \cdot \vec{x} + \omega_p t)} U(\vec{p}, \alpha) + d^\dagger(\vec{p}, \alpha) e^{-i(-\vec{p} \cdot \vec{x} + \omega_p t)} U(\vec{p}, \alpha) \right]$$

demanding the commutation (ref: Greiner & Ryder):

$$\{\psi_a(\vec{x}, t), \psi_b^\dagger(\vec{y}, t)\} = \delta_{ab} \tilde{\delta}(\vec{x} - \vec{y})$$

With commutation of annihilation & creation operator:

$$\left\{ b(\vec{p}, \alpha), b^\dagger(\vec{q}, \beta) \right\} = (2\pi)^3 \delta_{\alpha\beta} \delta(\vec{p} - \vec{q}) = \left\{ d(\vec{p}, \alpha), d^\dagger(\vec{q}, \beta) \right\}$$

left-hand side:

$$\begin{aligned} \{\psi_a(\vec{x}, t), \psi_b^\dagger(\vec{y}, t)\} &= \sum_{\alpha, \beta} \int \frac{d^3 p \, d^3 q \, N_p N_q}{(2\pi)^6 (1+p^2)(1+q^2)} \left[ (2\pi)^3 \delta_{\alpha\beta} \delta(\vec{p} - \vec{q}) U_a(\vec{p}, \alpha) U_b^\dagger(\vec{q}, \beta) \right. \\ &\quad \left. e^{i(\vec{q} \cdot \vec{y} - \vec{p} \cdot \vec{x})} e^{i(\omega_p - \omega_q)t} \right. \\ &\quad \left. + (2\pi)^3 \delta_{\alpha\beta} U_a(\vec{p}, \alpha) U_b^\dagger(\vec{q}, \beta) \delta(\vec{p} - \vec{q}) \right. \\ &\quad \left. e^{i(\vec{q} \cdot \vec{x} - \vec{p} \cdot \vec{y})} e^{i(\omega_q - \omega_p)t} \right] \end{aligned}$$

$$\{\psi_a(\vec{x}, t), \psi_b^\dagger(\vec{y}, t)\} = \sum_{\alpha} \int \frac{d^3 p}{(2\pi)^3} \frac{N_p^2}{(1+p^2)^2} \left[ U_a(\vec{r}, \alpha) U_b^\dagger(\vec{r}, \alpha) e^{i\vec{r} \cdot (\vec{x} - \vec{y})} + U_a(\vec{r}, \alpha) U_b^\dagger(\vec{r}, \alpha) e^{i\vec{r} \cdot \vec{y}} \right]$$

$$= \int \frac{d^3 p}{(2\pi)^3} \frac{N_p^2}{(1+p^2)^2} e^{i\vec{r} \cdot \Delta \vec{x}} \left[ \sum_{\alpha} (U_a(\vec{r}, \alpha) U_b^\dagger(\vec{r}, \alpha) + U_a(\vec{r}, \alpha) U_b^\dagger(\vec{r}, \alpha)) \right]$$

$$= \int \frac{d^3 p}{(2\pi)^3} \frac{N_p^2}{(1+p^2)^2} \left[ 2 \delta_{ab} \right] e^{i\vec{r} \cdot (\vec{x} - \vec{y})}$$

$$= 2 \int \frac{d^3 p}{(2\pi)^3} \frac{N_p^2}{(1+p^2)^2} e^{i\vec{r} \cdot (\vec{x} - \vec{y})}$$

Since r.h.s :

$$\{\psi_a(\vec{x}, t), \psi_b^\dagger(\vec{y}, t)\} = \delta_{ab} \delta(\vec{x} - \vec{y})$$

$$= \delta_{ab} \int \frac{d^3 p}{(2\pi)^3} \frac{1}{(1+p^2)^2} e^{i\vec{r} \cdot (\vec{x} - \vec{y})}$$

So we have  $2N_p^2 = 1$  or  $N_p = \frac{1}{\sqrt{2}}$

accordingly:

$$\psi(\vec{x}, t) = \sum_{\alpha} \int \frac{d^3 p}{(1+p^2) (2\pi)^3 \sqrt{2}} \left[ b(\vec{r}, \alpha) e^{i\vec{r} \cdot \vec{x}_n} U(\vec{r}, \alpha) + d^\dagger(\vec{r}, \alpha) e^{-i\vec{r} \cdot \vec{x}_n} U(\vec{r}, \alpha) \right]$$

(3)

7.)  $\sigma\omega$  Lagrangian

$$\mathcal{L} = \bar{\Psi} \left[ i \gamma^n (\partial_n + i g_\omega \omega_n) - \left( m - \overbrace{g_\sigma}^{m^*} \sigma \right) \right] \Psi \\ + \frac{1}{2} \left[ (\partial_n \sigma)^2 - m_\sigma^2 \sigma^2 \right] - \frac{1}{4} \omega_{\mu\nu} \omega^{\mu\nu} + \frac{1}{2} m_\omega^2 \omega_\mu \omega^\mu$$

in the mean relativistic scheme:

7.1) Dirac equation for nucleon

$$\left[ \gamma_n (i \partial^n - g_\omega \omega^n) - (m - g_\sigma \sigma) \right] \psi(x) = 0 \quad \dots (7.1)$$

denote  $\psi(x)$  spinor expand in maximally localized state

7.2) Condition for meson  $\sigma\omega$  (under MRF scheme):

$$m_\sigma^2 \langle \sigma \rangle = g_\sigma \langle \bar{\Psi} \Psi \rangle$$

$$m_\omega^2 \langle \omega_0 \rangle = g_\omega \langle \psi^\dagger \psi \rangle \quad \dots (7.2)$$

$$m_\omega^2 \langle \omega_k \rangle = g_\omega \langle \bar{\Psi} \gamma_k \Psi \rangle = 0$$

(9)



## 8.) Equation of State

8.1) Scalar density  $\rho_s = \langle \bar{\psi} \psi \rangle$

$$\begin{aligned}
 \langle \bar{\psi} \psi \rangle &= \sum_{\alpha\beta} \int \frac{d^3p \, d^3q}{(1+\beta p^2)(1+\beta q^2)(2\pi)^3 2} \bar{U}(\vec{p}, \alpha) U(\vec{q}, \beta) e^{iX^h(\vec{p}_n - \vec{q}_n)} \delta(\vec{p} - \vec{q}) \delta_{\alpha\beta} \\
 &= \int \frac{d^3p}{2(2\pi)^3 (1+\beta p^2)^2} \sum_{\alpha} \bar{U}(\vec{p}, \alpha) U(\vec{p}, \alpha) \\
 &= \int \frac{d^3p}{(2\pi)^3 (1+\beta p^2)^2} \frac{m^*}{\omega_p} \\
 &= \int \frac{d^3p}{(2\pi)^3 (1+\beta p^2)^2} \frac{m - g_\sigma \sigma}{\sqrt{\vec{p}^2 + m^{*2}}} \\
 &= \int \frac{d^3p}{(2\pi)^3 (1+\beta p^2)^2} \frac{m - g_\sigma \sigma}{\left[ \frac{1}{\beta} (\tan^{-1} \sqrt{\beta} p)^2 + (m - g_\sigma \sigma)^2 \right]^{1/2}}
 \end{aligned}$$

$$\rho_s = \langle \bar{\psi} \psi \rangle = \frac{1}{2\pi^2} \int_0^{p_F} \frac{p^2 dp}{(1+\beta p^2)^2} \frac{m - g_\sigma \sigma}{\left[ \frac{1}{\beta} (\tan^{-1} \sqrt{\beta} p)^2 + (m - g_\sigma \sigma)^2 \right]^{1/2}}$$

... (8.1)

Scalar density

(8.2) Vector density  $\rho_0 = \langle \psi^\dagger \psi \rangle$

$$\langle \psi^\dagger \psi \rangle = \sum_{\alpha, \beta} \int \frac{d^3 p \, d^3 q}{2(2\pi)^3 (1+\beta p^2)(1+\beta q^2)} U^\dagger(\vec{p}, \alpha) U(\vec{q}, \beta) e^{i x^n (\vec{p}_n - \vec{q}_n)} \delta(\vec{p} - \vec{q}) \delta_{\alpha, \beta}$$

$$= \int \frac{d^3 p}{2(2\pi)^3 (1+\beta p^2)^2} \sum_{\alpha} \underbrace{U^\dagger(\vec{p}, \alpha) U(\vec{p}, \alpha)}_2$$

$$= \int \frac{d^3 p}{(2\pi)^3 (1+\beta p^2)^2}$$

$$= \frac{1}{2\pi^2} \int_0^{p_f} \frac{p^2 \, dp}{(1+\beta p^2)^2}$$

$$= \frac{1}{2\pi^2} \left[ \frac{\tan^{-1}[\sqrt{\beta} p_f] - \frac{\sqrt{\beta} p_f}{1+\beta p_f^2}}{2\beta^{3/2}} \right]$$

$$\rho_0 = \langle \psi^\dagger \psi \rangle = \frac{1}{4\pi^2 (1+\beta p_f^2) \beta^{3/2}} \left[ (1+\beta p_f^2) \tan^{-1}(\sqrt{\beta} p_f) - \sqrt{\beta} p_f \right]$$

--- (8.2)

Vector density

### 8.3) Energy density

menggunakan bentuk (7.156) dari Glendenning :

$$\epsilon = - \langle \mathcal{L} \rangle + \langle \bar{\psi} \gamma_0 k_0 \psi \rangle$$

with

$$k_0 = g_\omega \omega_0 + \omega_p = g_\omega \omega_0 + \sqrt{\vec{p}^2 + m^*{}^2}$$

↳:

$$(a) \langle \bar{\psi} \gamma_0 k_0 \psi \rangle = \langle \psi^\dagger k_0 \psi \rangle$$

$$= \frac{1}{2\pi^2} \int_0^{p_F} \frac{p^2 dp}{(1 + \beta p^2)^2} \left[ g_\omega \omega_0 + \sqrt{\vec{p}^2 + m^*{}^2} \right]$$

$$= g_\omega \omega_0 \langle \psi^\dagger \psi \rangle + \frac{1}{2\pi^2} \int_0^{p_F} p^2 \sqrt{\frac{1}{\beta} (\tan^{-1} \sqrt{\beta} p)^2 + m^*{}^2} dp$$

$$(b) \langle \mathcal{L} \rangle = -\frac{1}{2} m_\sigma^2 \sigma^2 + \frac{1}{2} m_\omega^2 \omega_0^2$$

accordingly from (7.2):

$$m_\omega^2 \omega_0 = g_\omega \langle \psi^\dagger \psi \rangle$$

$$m_\omega^2 \omega_0^2 = g_\omega \omega_0 \langle \psi^\dagger \psi \rangle$$

↳

$$\epsilon = - \langle \mathcal{L} \rangle + \langle \bar{\psi} \gamma_0 k_0 \psi \rangle$$

$$\epsilon = \frac{1}{2} m_\sigma^2 \sigma^2 + \frac{1}{2} m_\omega^2 \omega_0^2 + \frac{1}{2\pi^2} \int_0^{p_F} p^2 \sqrt{\frac{1}{\beta} (\tan^{-1} \sqrt{\beta} p)^2 + (m - g_\sigma \sigma)^2} dp$$

⑦

energy density

--- (8.5)

8.3) pressure

$$P = \langle \mathcal{L} \rangle + \frac{1}{3} \langle \bar{\psi} \gamma_i k_i \psi \rangle$$

$$= -\frac{1}{2} m_\sigma^2 \sigma^2 + \frac{1}{2} m_\omega^2 \omega_0^2 + \frac{1}{6\pi^2} \int_0^{p_F} \frac{p^2 dp}{(1+\beta p^2)^2} \frac{\bar{P}^2}{\sqrt{\bar{P}^2 + m^{*2}}}$$

$$P = -\frac{1}{2} m_\sigma^2 \sigma^2 + \frac{1}{2} m_\omega^2 \omega_0^2 + \frac{1}{6\pi^2} \int_0^{p_F} \frac{p^2 dp}{(1+\beta p^2)^2} \frac{\frac{1}{\beta} (\tan^{-1} \sqrt{\beta} p)^2}{\left[ \frac{1}{\beta} (\tan^{-1} \sqrt{\beta} p)^2 + m^{*2} \right]^{1/2}}$$

$$P = -\frac{1}{2} m_\sigma^2 \sigma^2 + \frac{1}{2} m_\omega^2 \omega_0^2 + \frac{1}{6\pi^2} \int_0^{p_F} \frac{p^2 (\tan^{-1}(\sqrt{\beta} p))^2}{\beta (1+\beta p^2)^2 \left[ \frac{1}{\beta} (\tan^{-1}(\sqrt{\beta} p))^2 + (m-\frac{1}{2}\sigma)^2 \right]^{1/2}}$$

pressure

d